NewEchoAll proof minor

examples/new_echo/NewEchoAll.v
@@ -9,68 +9,45 @@ Require Import PCM.
 Require Import Hoare.
 Require Import MutHeader SimModSem.
 Require Import OpenDef.
-Require Import Mem0 NewStack0 NewEcho0 NewEchoMain0 NewClient0.
-
+Require Import Mem0 NewStack3A NewStack0 NewEcho0 NewEchoMain0 NewClient0.
 
 Set Implicit Arguments.
 
 
+Definition EchoGRA: GRA.t := GRA.of_list [Mem1.memRA; stkRA].
+Local Existing Instance EchoGRA.
+
+Instance memRA_inG: @GRA.inG Mem1.memRA EchoGRA.
+Proof.
+  exists 0. ss.
+Qed.
+Local Existing Instance memRA_inG.
+
+Instance stkRA_inG: @GRA.inG stkRA EchoGRA.
+Proof.
+  exists 1. ss.
+Qed.
+Local Existing Instance stkRA_inG.
+
 
 
 Section ECHOIMPL.
-
-  Let Σ: GRA.t := GRA.of_list [].
-  Local Existing Instance Σ.
-
   Definition echo_impl: ModL.t :=
     Mod.add_list [Mem; Stack; Echo; Main; Client].
-
+  Definition echo_impl_itr := ModSemL.initial_itr (ModL.enclose echo_impl) None.
 End ECHOIMPL.
-
-Definition echo_impl_itr := ModSemL.initial_itr (ModL.enclose echo_impl) None.
-
-
 
 
 Require Import Mem0 NewStackImp NewEchoImp NewEchoMainImp NewClientImp.
-
 Section ECHOIMP.
-
-  Let Σ: GRA.t := GRA.of_list [].
-  Local Existing Instance Σ.
-
   Definition echo_imp: ModL.t :=
     Mod.add_list [Mem; Stack; Echo; EchoMain; Client].
-
+  Definition echo_imp_itr := ModSemL.initial_itr (ModL.enclose echo_imp) None.
 End ECHOIMP.
-
-Definition echo_imp_itr := ModSemL.initial_itr (ModL.enclose echo_imp) None.
-
 
 
 Require Import MemOpen NewStack3A NewEcho1 NewEchoMain0 NewClient0.
-Require Import NewEchoMainImp0proof NewStackImp0proof NewEchoImp0proof NewClientImp0proof NewStack01proof NewStack12proof NewStack23Aproof NewEcho01proof.
-Require Import SimModSem.
-Require Import Mem0Openproof MemOpen0proof.
-Require Import Open.
-
 Section ECHOSPEC.
-
-  Let Σ: GRA.t := GRA.of_list [Mem1.memRA; stkRA].
-  Local Existing Instance Σ.
-
-  Let memRA_inG: @GRA.inG Mem1.memRA Σ.
-  Proof.
-    exists 0. ss.
-  Qed.
-  Local Existing Instance memRA_inG.
-
-  Let stkRA_inG: @GRA.inG stkRA Σ.
-  Proof.
-    exists 1. ss.
-  Qed.
-  Local Existing Instance stkRA_inG.
-
   Let frds: list string := ["Stack"; "Echo"].
   Definition echo_spec: ModL.t :=
     Mod.add_list [
@@ -81,78 +58,85 @@ Section ECHOSPEC.
       Client
       ].
 
-  Lemma refines2_cons mhd0 mhd1 mtl0 mtl1
-        (HD: refines2 [mhd0] [mhd1])
-        (TL: refines2 mtl0 mtl1)
-    :
-      refines2 (mhd0::mtl0) (mhd1::mtl1).
-  Proof.
-  Admitted.
+  Definition echo_spec_itr := ModSemL.initial_itr (ModL.enclose echo_spec) None.
+End ECHOSPEC.
 
-  Lemma refines2_app mhd0 mhd1 mtl0 mtl1
-        (HD: refines2 mhd0 mhd1)
-        (TL: refines2 mtl0 mtl1)
-    :
-      refines2 (mhd0++mtl0) (mhd1++mtl1).
-  Proof.
-  Admitted.
 
-  Section PROOF.
-    Theorem echo_correct:
-      refines echo_imp echo_spec.
-    Proof.
-      unfold echo_imp, echo_spec. transitivity echo_impl.
-      { eapply refines2_pairwise. econs.
-        { ss. }
-        econs.
-        { eapply adequacy_local2. eapply NewStackImp0proof.correct. }
-        econs.
-        { eapply adequacy_local2. eapply NewEchoImp0proof.correct. }
-        econs.
-        { eapply adequacy_local2. eapply NewEchoMainImp0proof.correct. }
-        econs.
-        { eapply adequacy_local2. eapply NewClientImp0proof.correct. }
-        ss.
-      }
-      unfold echo_impl.
-      pose (kmd0 := [KMem; NewStack1.KStack]).
-      transitivity (Mod.add_list (KMod.transl_tgt_list kmd0 ++ [NewEcho0.Echo; NewEchoMain0.Main; Client])).
-      { eapply refines2_cons.
-        { eapply adequacy_local2. eapply Mem0Openproof.correct. }
-        eapply refines2_cons.
-        { eapply adequacy_local2. eapply NewStack01proof.correct. i.
-          etrans; [|eapply to_closed_stb_weaker].
-          stb_incl_tac; tauto. }
-        refl.
-      }
-      etrans.
-      { rewrite Mod.add_list_app. eapply refines_proper_r.
-        eapply adequacy_open. i. exists ε. split.
-        { admit "URA wf". }
-        { ii. ss. }
-      }
-      pose (kmd1 := [NewStack3A.KStack; KEcho]).
-      transitivity (Mod.add_list (Mem0.Mem :: (KMod.transl_tgt_list kmd1) ++ [Main; Client])).
-      { rewrite <- Mod.add_list_app. eapply refines2_cons.
-        { eapply adequacy_local2. eapply MemOpen0proof.correct. }
-        eapply refines2_cons.
-        { etrans.
-          { eapply adequacy_local2. eapply NewStack12proof.correct. }
-          { eapply adequacy_local2. eapply NewStack23Aproof.correct. }
-        }
-        eapply refines2_cons.
-        { eapply adequacy_local2. eapply NewEcho01proof.correct.
-          stb_context_incl_tac; tauto. }
-        refl.
-      }
-      eapply refines2_cons; [refl|].
-      transitivity (KMod.transl_src_list kmd1 ++ [Main; Client]); [|refl].
-      eapply refines2_app; [|refl].
+Lemma refines2_cons mhd0 mhd1 mtl0 mtl1
+      (HD: refines2 [mhd0] [mhd1])
+      (TL: refines2 mtl0 mtl1)
+  :
+    refines2 (mhd0::mtl0) (mhd1::mtl1).
+Proof.
+Admitted.
+
+Lemma refines2_app mhd0 mhd1 mtl0 mtl1
+      (HD: refines2 mhd0 mhd1)
+      (TL: refines2 mtl0 mtl1)
+  :
+    refines2 (mhd0++mtl0) (mhd1++mtl1).
+Proof.
+Admitted.
+
+Require Import NewEchoMainImp0proof NewStackImp0proof NewEchoImp0proof NewClientImp0proof NewStack01proof NewStack12proof NewStack23Aproof NewEcho01proof.
+Require Import SimModSem.
+Require Import Mem0Openproof MemOpen0proof.
+Require Import Open.
+
+
+Section PROOF.
+  Theorem echo_correct:
+    refines echo_imp echo_spec.
+  Proof.
+    unfold echo_imp, echo_spec. transitivity echo_impl.
+    { eapply refines2_pairwise. econs.
+      { ss. }
+      econs.
+      { eapply adequacy_local2. eapply NewStackImp0proof.correct. }
+      econs.
+      { eapply adequacy_local2. eapply NewEchoImp0proof.correct. }
+      econs.
+      { eapply adequacy_local2. eapply NewEchoMainImp0proof.correct. }
+      econs.
+      { eapply adequacy_local2. eapply NewClientImp0proof.correct. }
+      ss.
+    }
+    unfold echo_impl.
+    pose (kmd0 := [KMem; NewStack1.KStack]).
+    transitivity (Mod.add_list (KMod.transl_tgt_list kmd0 ++ [NewEcho0.Echo; NewEchoMain0.Main; Client])).
+    { eapply refines2_cons.
+      { eapply adequacy_local2. eapply Mem0Openproof.correct. }
+      eapply refines2_cons.
+      { eapply adequacy_local2. eapply NewStack01proof.correct. i.
+        etrans; [|eapply to_closed_stb_weaker].
+        stb_incl_tac; tauto. }
+      refl.
+    }
+    etrans.
+    { rewrite Mod.add_list_app. eapply refines_proper_r.
       eapply adequacy_open. i. exists ε. split.
       { admit "URA wf". }
       { ii. ss. }
-    Qed.
-  End PROOF.
-End ECHOSPEC.
-
-Definition echo_spec_itr := ModSemL.initial_itr (ModL.enclose echo_spec) None.
+    }
+    pose (kmd1 := [NewStack3A.KStack; KEcho]).
+    transitivity (Mod.add_list (Mem0.Mem :: (KMod.transl_tgt_list kmd1) ++ [Main; Client])).
+    { rewrite <- Mod.add_list_app. eapply refines2_cons.
+      { eapply adequacy_local2. eapply MemOpen0proof.correct. }
+      eapply refines2_cons.
+      { etrans.
+        { eapply adequacy_local2. eapply NewStack12proof.correct. }
+        { eapply adequacy_local2. eapply NewStack23Aproof.correct. }
+      }
+      eapply refines2_cons.
+      { eapply adequacy_local2. eapply NewEcho01proof.correct.
+        stb_context_incl_tac; tauto. }
+      refl.
+    }
+    eapply refines2_cons; [refl|].
+    transitivity (KMod.transl_src_list kmd1 ++ [Main; Client]); [|refl].
+    eapply refines2_app; [|refl].
+    eapply adequacy_open. i. exists ε. split.
+    { admit "URA wf". }
+    { ii. ss. }
+  Qed.
+End PROOF.
